NormalizationExists.v
@@ -6,40 +6,66 @@ Require Export SystemFR.ScalaDepSugar.
 
 Opaque reducible_values.
 
-(*
-Lemma open_equivalent_types_trans: forall Θ Γ T1 T2 T3,
-  [ Θ; Γ ⊨ open 0 S t = S' ] ->
-  [ Θ; Γ ⊨ T_exists (T_singleton T t) S = S' ].
+Lemma nexists_1: forall ρ s S S' T T',
+  valid_interpretation ρ ->
+  is_erased_type T ->
+  is_erased_type T' ->
+  wf T 1 ->
+  wf T' 0 ->
+  pfv T term_var = nil ->
+  pfv T' term_var = nil ->
+  [ ρ | s : S ] ->
+  [ ρ | S = S' ] ->
+  (forall a, [ ρ | a : S' ]v -> [ ρ | open 0 T a = T' ]) ->
+  [ ρ | T_exists S T = T' ].
 Proof.
-*)
-(*
-Lemma open_nexists: forall Θ Γ S T t,
-  [ Θ; Γ ⊨ t : T ] ->
-  [ Θ; Γ ⊨ T_exists (T_singleton T t) S = open 0 S t ].
-Proof.
-Admitted.
-*)
+  intros; unfold equivalent_types;
+    repeat step || simp_red || rewrite reducibility_rewrite;
+    t_closer;
+    eauto using equivalent_types_reducible_values.
 
-Lemma nexists_1: forall ρ T t U T',
-  (forall v, [ ρ | v : T_singleton U t ]v -> [ ρ | open 0 T v = T' ]) ->
-  [ ρ | T_exists (T_singleton U t) T = T' ].
-Proof.
-  repeat step || simp_red.
-Admitted.
+ unfold reducible, reduces_to in H6; steps.
+ exists v0; steps; eauto with wf fv erased;
+   eauto using equivalent_types_reducible_values, equivalent_types_reducible_values_back.
+Qed.
 
-Lemma open_nexists_1_helper: forall Θ Γ T t U T' x,
-(*  [ Θ; Γ ⊨ t : T ] -> ?? *)
-  [ Θ; (x, T_singleton U t) :: Γ ⊨ T = T' ] ->
-  [ Θ; Γ ⊨ T_exists (T_singleton U t) T = T' ].
+Lemma open_nexists_1_helper: forall Θ Γ s S S' T T' x,
+  is_erased_type T ->
+  is_erased_type T' ->
+  wf T 1 ->
+  wf T' 0 ->
+  subset (fv T) (support Γ) ->
+  subset (fv T') (support Γ) ->
+  ~ x ∈ pfv S' term_var ->
+  ~ x ∈ pfv T' term_var ->
+  ~ x ∈ pfv_context Γ term_var ->
+  [ Θ; Γ ⊨ s : S ] ->
+  [ Θ; Γ ⊨ S = S' ] ->
+  [ Θ; (x, S') :: Γ ⊨ open 0 T (fvar x term_var) = T' ] ->
+  [ Θ; Γ ⊨ T_exists S T = T' ].
 Proof.
-Admitted.
+  unfold open_reducible, open_equivalent_types; repeat step || eapply nexists_1; t_closer.
 
-Lemma open_nexists_1: forall Γ T t U T' x,
-(*  [ Θ; Γ ⊨ t : T ] -> ?? *)
-  [ (x, T_singleton U t) :: Γ ⊨ T = T' ] ->
-  [ Γ ⊨ T_exists (T_singleton U t) T = T' ].
+  unshelve epose proof (H10 ρ ((x, a) :: l) _ _ _);
+    repeat step || apply SatCons || t_substitutions; t_closer.
+Qed.
+
+Lemma open_nexists_1: forall Γ s S S' T T' x,
+  is_erased_type T ->
+  is_erased_type T' ->
+  wf T 1 ->
+  wf T' 0 ->
+  subset (fv T) (support Γ) ->
+  subset (fv T') (support Γ) ->
+  ~ x ∈ pfv S' term_var ->
+  ~ x ∈ pfv T' term_var ->
+  ~ x ∈ pfv_context Γ term_var ->
+  [ Γ ⊨ s : S ] -> (* algorithm invariant: every type is inhabited *)
+  [ Γ ⊨ S = S' ] ->
+  [ (x, S') :: Γ ⊨ open 0 T (fvar x term_var) = T' ] ->
+  [ Γ ⊨ T_exists S T = T' ].
 Proof.
-  intros; eauto using open_nexists_1_helper.
+  eauto using open_nexists_1_helper.
 Qed.
 
 Lemma nexists_2: forall ρ S S' T T',
@@ -54,8 +80,7 @@ Lemma nexists_2: forall ρ S S' T T',
   (forall a, [ ρ | a : S' ]v -> [ ρ | open 0 T a = open 0 T' a ]) ->
   [ ρ | T_exists S T = T_exists S' T' ].
 Proof.
-  intros.
-  unfold equivalent_types;
+  intros; unfold equivalent_types;
     repeat step || simp_red || rewrite reducibility_rewrite;
     t_closer.
 
