NormalizationMatch.v
@@ -2,47 +2,516 @@ Require Import PeanoNat.
 
 Require Export SystemFR.NormalizationSing.
 Require Export SystemFR.SubtypeList.
+Require Export SystemFR.InferMatch.
 
-Lemma open_nmatch_3: forall Θ Γ T2 T3 t t',
+Opaque reducible_values.
+
+Lemma open_nmatch_3: forall Γ T2 T3 t t',
+  is_erased_type T2 ->
+  is_erased_type T3 ->
+  wf T2 0 ->
+  wf T3 2 ->
+  subset (fv T2) (support Γ) ->
+  subset (fv T3) (support Γ) ->
   [ Γ ⊨ t ⤳* t' ] ->
-  [ Θ; Γ ⊨ List_Match t T2 T3 = List_Match t' T2 T3 ].
+  [ Γ ⊨ List_Match t T2 T3 = List_Match t' T2 T3 ].
 Proof.
-Admitted.
+  eauto using open_sub_list_match_scrut, delta_beta_obs_equiv.
+Qed.
+
+Lemma nmatch_nil: forall ρ T2 T3,
+  valid_interpretation ρ ->
+  [ ρ | List_Match tnil T2 T3 = T2 ].
+Proof.
+  unfold equivalent_types, List_Match;
+    repeat step || simp_red_top_level_goal || simp_red_top_level_hyp || open_none;
+    eauto using reducible_values_closed.
+
+  - apply_anywhere equivalent_value_left; steps; eauto with closing values.
+  - left; repeat step || simp_red || exists uu;
+      eauto using reducible_values_closed;
+      eauto using equivalent_refl.
+Qed.
+
+Lemma right_left_star_helper:
+  forall t1 t2,
+    star scbv_step t1 t2 ->
+    forall t1' t2',
+      t1 = tright t1' ->
+      t2 = tleft t2' ->
+      False.
+Proof.
+  induction 1; repeat step || t_invert_step; eauto.
+Qed.
+
+Lemma right_left_star:
+  forall t1 t2,
+    star scbv_step (tright t1) (tleft t2) ->
+    False.
+Proof.
+  eauto using right_left_star_helper.
+Qed.
+
+Lemma right_right_star_helper:
+  forall t1 t2,
+    star scbv_step t1 t2 ->
+    forall t1' t2',
+      t1 = tright t1' ->
+      t2 = tright t2' ->
+      star scbv_step t1' t2'.
+Proof.
+  induction 1; repeat step || t_invert_step; eauto with star.
+Qed.
+
+Lemma right_right_star:
+  forall t1 t2,
+    star scbv_step (tright t1) (tright t2) ->
+    star scbv_step t1 t2.
+Proof.
+  eauto using right_right_star_helper.
+Qed.
+
+Lemma left_left_star_helper:
+  forall t1 t2,
+    star scbv_step t1 t2 ->
+    forall t1' t2',
+      t1 = tleft t1' ->
+      t2 = tleft t2' ->
+      star scbv_step t1' t2'.
+Proof.
+  induction 1; repeat step || t_invert_step; eauto with star.
+Qed.
+
+Lemma left_left_star:
+  forall t1 t2,
+    star scbv_step (tleft t1) (tleft t2) ->
+    star scbv_step t1 t2.
+Proof.
+  eauto using left_left_star_helper.
+Qed.
+
+Lemma equivalent_err:
+  forall v,
+    cbv_value v ->
+    [ v ≡ notype_err ] ->
+    False.
+Proof.
+  intros.
+  equivalence_instantiate (app (notype_lambda ttrue) (lvar 0 term_var)); steps.
+  unshelve epose proof (H3 _); eauto using scbv_step_same, star_one with smallstep;
+    repeat step || t_invert_star || step_inversion cbv_value.
+Qed.
+
+Lemma right_left_equivalence:
+  forall t v,
+    cbv_value v ->
+    [ tright t ≡ tleft v ] ->
+    False.
+Proof.
+  intros.
+  unshelve epose proof (equivalent_context (sum_match (lvar 0 term_var) ttrue notype_err)
+  _ _ _ _ _ H0) as HH1; steps.
+  apply equivalent_sym in HH1.
+  unshelve epose proof (equivalent_normalizing _ _ ttrue HH1 _ _);
+    repeat step || t_invert_star;
+    eauto using scbv_step_same, star_one with smallstep values;
+    eauto using right_left_star;
+    eauto using equivalent_err with values.
+Qed.
+
+Lemma tright_equiv:
+  forall t v,
+    cbv_value v ->
+    [ tright t ≡ tright v ] ->
+    [ t ≡ v ].
+Proof.
+  intros.
+  unshelve epose proof (equivalent_context (sum_match (lvar 0 term_var) notype_err (lvar 0 term_var))
+  _ _ _ _ _ H0) as HH1; steps.
+  apply equivalent_sym in HH1.
+  unshelve epose proof (equivalent_normalizing _ _ v HH1 _ _);
+    eauto using scbv_step_same, star_one with smallstep;
+    repeat step || t_invert_star || step_inversion cbv_value;
+    eauto with values;
+    try solve [ eexists; steps ].
+
+  eapply equivalent_trans; eauto using equivalent_sym.
+  apply_anywhere right_right_star.
+  apply equivalent_trans with v'; equivalent_star.
+Qed.
+
+Lemma tleft_equiv:
+  forall t v,
+    cbv_value v ->
+    [ tleft t ≡ tleft v ] ->
+    [ t ≡ v ].
+Proof.
+  intros.
+  unshelve epose proof (equivalent_context (sum_match (lvar 0 term_var) (lvar 0 term_var) notype_err)
+  _ _ _ _ _ H0) as HH1; steps.
+  apply equivalent_sym in HH1.
+  unshelve epose proof (equivalent_normalizing _ _ v HH1 _ _);
+    eauto using scbv_step_same, star_one with smallstep;
+    repeat step || t_invert_star || step_inversion cbv_value;
+    eauto with values;
+    try solve [ eexists; steps ].
+
+  eapply equivalent_trans; eauto using equivalent_sym.
+  apply_anywhere left_left_star.
+  apply equivalent_trans with v'; equivalent_star.
+Qed.
+
+Lemma reducibility_open_equivalent2:
+  forall T t1 t2 t1' t2' ρ v,
+    [ ρ | v : open 0 (open 1 T t1) t2 ]v  ->
+    valid_interpretation ρ ->
+    is_erased_type T ->
+    wf T 2 ->
+    pfv T term_var = nil ->
+    [ t1 ≡ t1' ] ->
+    [ t2 ≡ t2' ] ->
+    [ ρ | v : open 0 (open 1 T t1') t2' ]v.
+Proof.
+  intros.
+  eapply reducibility_open_equivalent; eauto; steps; eauto with erased wf fv.
+  rewrite swap_term_holes_open in * by (
+    unfold equivalent_terms; repeat step || destruct_and; t_closer
+  ).
+  eapply reducibility_open_equivalent; eauto; steps; eauto with erased wf fv.
+Qed.
+
+Opaque List.
+
+Lemma pair_equiv_1:
+  forall t1 t2 v1 v2,
+    [ pp t1 t2 ≡ pp v1 v2 ] ->
+    cbv_value v1 ->
+    cbv_value v2 ->
+    [ t1 ≡ v1 ].
+Proof.
+  intros.
+  unshelve epose proof (equivalent_context (pi1 (lvar 0 term_var)) _ _ _ _ _ H) as HH; steps.
+  apply equivalent_sym in HH.
+  unshelve epose proof (equivalent_normalizing _ _ v1 HH _ _);
+    eauto using scbv_step_same, star_one with smallstep;
+    repeat step || t_invert_star || step_inversion cbv_value;
+    eauto with values;
+    try solve [ eexists; steps ].
+  eapply equivalent_trans; eauto using equivalent_sym; equivalent_star.
+Qed.
+
+Lemma pair_equiv_2:
+  forall t1 t2 v1 v2,
+    [ pp t1 t2 ≡ pp v1 v2 ] ->
+    cbv_value v1 ->
+    cbv_value v2 ->
+    [ t2 ≡ v2 ].
+Proof.
+  intros.
+  unshelve epose proof (equivalent_context (pi2 (lvar 0 term_var)) _ _ _ _ _ H) as HH; steps.
+  apply equivalent_sym in HH.
+  unshelve epose proof (equivalent_normalizing _ _ v2 HH _ _);
+    eauto using scbv_step_same, star_one with smallstep;
+    repeat step || t_invert_star || step_inversion cbv_value;
+    eauto with values;
+    try solve [ eexists; steps ].
+  eapply equivalent_trans; eauto using equivalent_sym; equivalent_star.
+Qed.
+
+Lemma nmatch_cons: forall ρ t ts T2 T3,
+  valid_interpretation ρ ->
+  wf t 0 ->
+  wf ts 0 ->
+  is_erased_term t ->
+  is_erased_term ts ->
+  pfv t term_var = nil ->
+  pfv ts term_var = nil ->
+  wf T3 2 ->
+  pfv T3 term_var = nil ->
+  is_erased_type T3 ->
+  [ ρ | t : T_top ] ->
+  [ ρ | ts : List ] ->
+  [ ρ | List_Match (tcons t ts) T2 T3 = open 0 (open 1 T3 t) ts ].
+Proof.
+  unfold equivalent_types, List_Match;
+    repeat step || simp_red_top_level_goal || simp_red_top_level_hyp || open_none;
+    eauto using reducible_values_closed;
+    eauto 3 using right_left_equivalence with exfalso values.
+
+  - apply_anywhere tright_equiv; eauto with closing values.
+    eapply reducibility_open_equivalent2; try eassumption; steps;
+      eauto 3 using equivalent_sym, pair_equiv_1, pair_equiv_2 with closing.
+
+  - right; repeat step.
+    apply reducible_expr_value; eauto with values.
+    apply reducible_exists with t;
+      repeat step || list_utils || rewrite open_list || open_none; eauto with fv wf erased.
+    apply reducible_exists with ts;
+      repeat step || list_utils || open_none; eauto with fv wf erased.
+    apply reducible_type_refine with uu; repeat step || open_none || list_utils;
+      eauto with fv wf erased;
+      eauto using reducible_value_expr.
+    apply reducible_value_expr; repeat step || simp_red_goal.
+    apply equivalent_refl; repeat step || list_utils.
+Qed.
+
+Opaque List_Match.
 
 Lemma open_nmatch_nil: forall Θ Γ T2 T3,
   [ Θ; Γ ⊨ List_Match tnil T2 T3 = T2 ].
 Proof.
-Admitted.
+  unfold open_equivalent_types; repeat step || rewrite substitute_List_Match;
+    eauto with wf;
+    eauto using nmatch_nil.
+Qed.
 
-Lemma open_nmatch_1: forall Θ Γ T2 T2' T3 t,
+Lemma open_nmatch_1: forall Γ T2 T2' T3 t,
+  is_erased_type T2 ->
+  is_erased_type T3 ->
+  wf T2 0 ->
+  wf T3 2 ->
+  subset (fv T2) (support Γ) ->
+  subset (fv T3) (support Γ) ->
   [ Γ ⊨ t ⤳* tnil ] ->
-  [ Θ; Γ ⊨ T2 = T2' ] ->
-  [ Θ; Γ ⊨ List_Match t T2 T3 = T2' ].
+  [ Γ ⊨ T2 = T2' ] ->
+  [ Γ ⊨ List_Match t T2 T3 = T2' ].
 Proof.
-Admitted.
+  intros.
+  eapply open_equivalent_types_trans; try apply open_nmatch_3;
+    eauto using open_equivalent_types_trans, open_nmatch_nil.
+Qed.
 
 Lemma open_nmatch_cons: forall Θ Γ T2 T3 t1 t2,
-  [ Θ; Γ ⊨ List_Match (tcons t1 t2) T2 T3 = open 0 (open 1 T3 t1) t2 ]. (* FIXME *)
+  wf t1 0 ->
+  wf t2 0 ->
+  wf T3 2 ->
+  is_erased_term t1 ->
+  is_erased_term t2 ->
+  is_erased_type T3 ->
+  subset (fv t1) (support Γ) ->
+  subset (fv t2) (support Γ) ->
+  subset (fv T3) (support Γ) ->
+  [ Θ; Γ ⊨ t1 : T_top ] ->
+  [ Θ; Γ ⊨ t2 : List ] ->
+  [ Θ; Γ ⊨ List_Match (tcons t1 t2) T2 T3 = open 0 (open 1 T3 t1) t2 ].
 Proof.
-Admitted.
+  unfold open_equivalent_types, open_reducible;
+    repeat step || rewrite substitute_List_Match || t_substitutions ||
+           t_instantiate_sat3 || apply nmatch_cons;
+    eauto with wf erased fv.
+Qed.
 
-(*
-Lemma open_normalization:
-  forall Θ Γ x T t S S',
-    lookup Nat.eq_dec Γ x = Some (T_singleton T t) ->
-    [ Θ; Γ ⊨ S = S' ] ->
-    ~ x ∈ fv S'.
-*)
+Lemma is_erased_term_close:
+  forall t k x,
+    is_erased_term t ->
+    is_erased_term (close k t x).
+Proof.
+  induction t; steps.
+Qed.
 
-Lemma open_nmatch_2: forall Θ Γ T2 T3 T3' t t1 t2 x y,
-  [ Γ ⊨ t ⤳* tcons t1 t2 ] ->
-  [ Θ; (x, T_singleton T_top t1) :: (y, T_singleton List t2) :: Γ ⊨
-    open 0 (open 1 T3 (fvar x term_var)) (fvar y term_var) = T3' ] -> (* FIXME *)
+Lemma is_erased_type_close:
+  forall T k x,
+    is_erased_type T ->
+    is_erased_type (close k T x).
+Proof.
+  induction T; steps; eauto using is_erased_term_close.
+Qed.
+
+Hint Resolve is_erased_term_close: erased.
+Hint Resolve is_erased_type_close: erased.
+
+Lemma reducibility_subst_equiv:
+  forall ρ v T x t1 t2,
+    [ ρ | v : psubstitute T ((x, t1) :: nil) term_var ]v ->
+    valid_interpretation ρ ->
+    wf T 0 ->
+    is_erased_type T ->
+    subset (fv T) (x :: nil) ->
+    [ t1 ≡ t2 ] ->
+    [ ρ | v : psubstitute T ((x, t2) :: nil) term_var ]v.
+Proof.
+  intros; repeat rewrite <- (open_close _ _ _ 0) in * by auto.
+  rewrite <- (open_close _ _ _ 0) in H by auto.
+  eapply reducibility_open_equivalent; eauto; repeat step;
+    eauto with erased wf;
+    eauto using fv_close_nil2.
+Qed.
+
+Lemma reducibility_subst_equiv2:
+  forall ρ T x t1 t2,
+    valid_interpretation ρ ->
+    wf T 0 ->
+    is_erased_type T ->
+    subset (fv T) (x :: nil) ->
+    [ t1 ≡ t2 ] ->
+    [ ρ | psubstitute T ((x, t1) :: nil) term_var = psubstitute T ((x, t2) :: nil) term_var ].
+Proof.
+  unfold equivalent_types; steps;
+    eauto using reducibility_subst_equiv, equivalent_sym.
+Qed.
+
+Lemma subset_diff:
+  forall s1 x s2,
+    subset s1 (x :: s2) ->
+    subset (s1 -- (x :: nil)) s2.
+Proof.
+  unfold subset; repeat step || instantiate_any || rewrite in_remove in *.
+Qed.
+
+Opaque diff.
+
+Lemma subset_diff2:
+  forall s1 x s2,
+    subset s1 (x :: s2) ->
+    subset (s1 -- s2) (x :: nil).
+Proof.
+  unfold subset; repeat step || instantiate_any || rewrite in_diff in *.
+Qed.
+
+Lemma closed_mapping_fv2:
+  forall l tag,
+    pclosed_mapping l tag ->
+    pfv_range l tag = nil.
+Proof.
+  induction l; repeat step || list_utils.
+Qed.
+
+Lemma reducibility_subst_equiv3:
+  forall ρ T x l t1 t2,
+    valid_interpretation ρ ->
+    wf T 0 ->
+    is_erased_type T ->
+    ~ x ∈ support l ->
+    wfs l 0 ->
+    erased_terms l ->
+    pclosed_mapping l term_var ->
+    subset (fv T) (x :: support l) ->
+    [ t1 ≡ t2 ] ->
+    [ ρ | psubstitute T ((x, t1) :: l) term_var = psubstitute T ((x, t2) :: l) term_var ].
+Proof.
+  intros.
+  repeat rewrite (substitute_cons4 _ T); steps.
+  apply reducibility_subst_equiv2; steps; eauto with wf erased fv.
+  eapply subset_transitive; eauto using fv_subst2;
+    repeat step || sets || rewrite closed_mapping_fv2 by auto;
+    eauto using subset_diff2;
+    eauto with sets.
+Qed.
+
+Lemma in_support_in_context:
+  forall P Γ l x,
+    x ∈ support l ->
+    satisfies P Γ l ->
+    x ∈ pfv_context Γ term_var.
+Proof.
+  intros; apply fv_context_support; erewrite satisfies_same_support; eauto.
+Qed.
+
+Lemma open_instantiate:
+  forall Θ Γ x t T T1 T2,
+    ~ x ∈ fv T ->
+    ~ x ∈ fv_context Γ ->
+    wf T1 0 ->
+    wf T2 0 ->
+    is_erased_type T1 ->
+    is_erased_type T2 ->
+    subset (fv T1) (x :: support Γ) ->
+    subset (fv T2) (x :: support Γ) ->
+    [ Θ; Γ ⊨ t : T ] ->
+    [ Θ; (x, T) :: Γ ⊨ T1 = T2 ] ->
+    [ Θ; Γ ⊨ psubstitute T1 ((x, t) :: nil) term_var = psubstitute T2 ((x, t) :: nil) term_var ].
+Proof.
+  unfold open_equivalent_types, open_reducible; repeat step || t_instantiate_sat3.
+  top_level_unfold reducible; top_level_unfold reduces_to; steps.
+  unshelve epose proof (H8 ρ ((x, v) :: l) _ _);
+    repeat step || apply SatCons || (rewrite <- substitute_cons3 by steps);
+    eauto with fv wf twf erased.
+
+  eapply equivalent_types_trans; try eapply reducibility_subst_equiv3;
+    repeat step || erewrite satisfies_same_support in * by eauto;
+    try solve [ equivalent_star ];
+    eauto using in_support_in_context;
+    eauto with wf erased fv.
+
+  eapply equivalent_types_trans; eauto; apply equivalent_types_sym.
+
+  apply reducibility_subst_equiv3;
+    repeat step || erewrite satisfies_same_support in * by eauto;
+    try solve [ equivalent_star ];
+    eauto using in_support_in_context;
+    eauto with wf erased fv.
+Qed.
+
+Lemma open_reducible_weaken:
+  forall Θ Γ x A t B,
+    ~ x ∈ fv t ->
+    ~ x ∈ fv B ->
+    [ Θ; Γ ⊨ t : B ] ->
+    [ Θ; (x, A) :: Γ ⊨ t : B ].
+Proof.
+  unfold open_reducible; repeat step || step_inversion satisfies || t_substitutions.
+Qed.
+
+Lemma open_nmatch_2: forall Γ T2 T3 T3' t t1 t2 x y,
+  is_erased_term t1 ->
+  is_erased_term t2 ->
+  is_erased_type T2 ->
+  is_erased_type T3 ->
+  is_erased_type T3' ->
+  wf t1 0 ->
+  wf t2 0 ->
+  wf T2 0 ->
+  wf T3 2 ->
+  wf T3' 0 ->
+  subset (fv t1) (support Γ) ->
+  subset (fv t2) (support Γ) ->
+  subset (fv T2) (support Γ) ->
+  subset (fv T3) (support Γ) ->
+  subset (fv T3') (support Γ) ->
+  ~ x ∈ fv t1 ->
+  ~ x ∈ fv t2 ->
+  ~ x ∈ fv T3 ->
   ~ x ∈ fv T3' ->
+  ~ x ∈ fv_context Γ ->
+  ~ y ∈ fv t1 ->
+  ~ y ∈ fv t2 ->
+  ~ y ∈ fv T3 ->
   ~ y ∈ fv T3' ->
-  [ Θ; Γ ⊨ List_Match t T2 T3 = T3' ].
+  ~ y ∈ fv_context Γ ->
+  x <> y ->
+  [ Γ ⊨ t1 : T_top ] ->
+  [ Γ ⊨ t2 : List ] ->
+  [ Γ ⊨ t ⤳* tcons t1 t2 ] ->
+  [ (x, T_singleton T_top t1) :: (y, T_singleton List t2) :: Γ ⊨
+    open 0 (open 1 T3 (fvar x term_var)) (fvar y term_var) = T3' ] ->
+  [ Γ ⊨ List_Match t T2 T3 = T3' ].
 Proof.
-Admitted.
+  intros.
+  eapply open_equivalent_types_trans; try apply open_nmatch_3; try eassumption; steps.
+  eapply open_equivalent_types_trans; try apply open_nmatch_cons; steps.
+  apply (open_instantiate _ _ _ t1) in H28;
+    repeat step || list_utils || apply wf_open || apply is_erased_type_open ||
+           rewrite pfv_shift2 in *;
+    eauto with fv wf erased;
+    eauto using subset_add2.
+  - apply (open_instantiate _ _ _ t2) in H28;
+      repeat step || list_utils || apply wf_open || apply wf_subst || t_substitutions ||
+             apply is_erased_type_open || apply subst_erased_type ||
+             rewrite pfv_shift2 in *;
+      eauto with fv wf erased;
+      eauto using subset_add2;
+      eauto using open_reducible_singleton.
 
+    + rewrite (substitute_nothing2 T3') in *; repeat step || rewrite substitute_nothing3 in *.
+      rewrite (substitute_nothing2 T3') in *; repeat step || rewrite substitute_nothing3 in *.
 
+    + eapply subset_transitive; eauto using fv_open; repeat step || sets.
+      eapply subset_transitive; eauto using fv_open; repeat step || sets;
+        eauto using subset_add2.
 
+  - eapply subset_transitive; eauto using fv_open; repeat step || sets.
+    eapply subset_transitive; eauto using fv_open; repeat step || sets;
+      eauto using subset_add2.
+  - apply open_reducible_weaken; repeat step || rewrite pfv_shift2 in *;
+      eauto using open_reducible_singleton.
+Qed.
