SubtypeNorm.v
@@ -1,0 +1,49 @@
+Require Export SystemFR.Untangle.
+Require Export SystemFR.InferApp.
+
+Lemma open_subnormwiden_helper:
+  forall Θ Γ T1 T1' T2,
+    widen T1 T1' ->
+    [ Θ; Γ ⊨ T1' <: T2 ] ->
+    [ Θ; Γ ⊨ T1  <: T2 ].
+Proof.
+  intros; eauto using widen_open_subtype, open_subtype_trans.
+Qed.
+
+Lemma open_subnormwiden:
+  forall Γ T1 T1' T2,
+    widen T1 T1' ->
+    [ Γ ⊨ T1' <: T2 ] ->
+    [ Γ ⊨ T1  <: T2 ].
+Proof.
+  eauto using open_subnormwiden_helper.
+Qed.
+
+Lemma open_subnorm_helper:
+  forall Θ Γ T1 T1' T1'' T2 T2' T2'',
+    [ Θ; Γ ⊨ T1 = T1' ] ->
+    [ Θ; Γ ⊨ T2 = T2' ] ->
+    untangle T1' T1'' ->
+    untangle T2' T2'' ->
+    [ Θ; Γ ⊨ T1'' <: T2'' ] ->
+    [ Θ; Γ ⊨ T1 <: T2 ].
+Proof.
+  intros.
+  eapply open_subtype_trans; eauto using open_equivalent_subtype.
+  eapply open_subtype_trans; eauto using open_equivalent_subtype, untangle_open_equivalent_types.
+  eapply open_subtype_trans; eauto.
+  eapply open_subtype_trans; eauto using open_equivalent_subtype_back.
+  eauto using open_equivalent_subtype_back, untangle_open_equivalent_types.
+Qed.
+
+Lemma open_subnorm:
+  forall Γ T1 T1' T1'' T2 T2' T2'',
+    [ Γ ⊨ T1 = T1' ] ->
+    [ Γ ⊨ T2 = T2' ] ->
+    untangle T1' T1'' ->
+    untangle T2' T2'' ->
+    [ Γ ⊨ T1'' <: T2'' ] ->
+    [ Γ ⊨ T1 <: T2 ].
+Proof.
+  eauto using open_subnorm_helper.
+Qed.
