Untangle.v
@@ -1,0 +1,12 @@
+Require Export SystemFR.ReducibilityLemmas.
+
+Inductive untangle: tree -> tree -> Prop :=
+| UntangleRefl: forall T, untangle T T
+.
+
+Lemma untangle_open_equivalent_types:
+  forall Θ Γ T1 T2,
+    untangle T1 T2 ->
+    [ Θ; Γ ⊨ T1 = T2 ].
+Proof.
+Admitted.
